wip

HumanEvalLean/HumanEval121.lean
@@ -1,5 +1,115 @@
-def solution : Unit :=
-  ()
+-- This can't be a module right now because `Rxi.Iterator.Monadic.Step` is not exposed
+import Std
+
+open Std Std.PRange
+
+def solution (xs : List Int) : Int :=
+  ((0 : Nat)...*).iter.zip xs.iter
+    |>.filter (fun (i, _) => i % 2 = 0)
+    |>.fold (init := 0) (fun sum (_, x) => sum + x)
+
+attribute [grind =] Iter.toList_take_zero Nat.succ?_eq
+
+public theorem Rxi.Iterator.toList_take_eq_match
+    [UpwardEnumerable α] [LawfulUpwardEnumerable α]
+    {it : Iter (α := Rxi.Iterator α) α} :
+    (it.take n).toList =  match n, it.internalState.next with
+      | 0, _ | _, none => []
+      | n + 1, some a =>
+          a :: ((⟨⟨UpwardEnumerable.succ? a⟩⟩ : Iter (α := Rxi.Iterator α) α).take n).toList := by
+  apply Eq.symm
+  simp only [Iter.toList_eq_match_step (it := it.take n), Iter.step_take]
+  cases n
+  · grind
+  · simp only
+    cases it.step using PlausibleIterStep.casesOn <;> rename_i heq
+    · rename_i it' _
+      rcases it with ⟨⟨next⟩⟩ | _
+      · simp [Iter.IsPlausibleStep, IterM.IsPlausibleStep, Iterator.IsPlausibleStep] at heq
+        simp [Rxi.Iterator.Monadic.step, Iter.toIterM] at heq -- ugly
+      · simp [Iter.IsPlausibleStep, IterM.IsPlausibleStep, Iterator.IsPlausibleStep] at heq
+        simp [Rxi.Iterator.Monadic.step, Iter.toIterM] at heq -- ugly
+        cases heq.2
+        cases it'
+        simp at heq
+        simp [heq]
+    · simp [Iter.IsPlausibleStep, IterM.IsPlausibleStep, Iterator.IsPlausibleStep] at heq
+      simp [Rxi.Iterator.Monadic.step, Iter.toIterM] at heq -- ugly
+      split at heq <;> contradiction
+    · simp [Iter.IsPlausibleStep, IterM.IsPlausibleStep, Iterator.IsPlausibleStep] at heq
+      simp [Rxi.Iterator.Monadic.step, Iter.toIterM] at heq -- ugly
+      split at heq
+      · simp [*]
+      · contradiction
+
+theorem Nat.toList_take_iter_rci_eq_match {m n : Nat} :
+    ((m...*).iter.take n).toList =
+      match n with
+      | 0 => []
+      | n + 1 => m :: (((m + 1)...*).iter.take n).toList := by
+  rw [Rxi.Iterator.toList_take_eq_match]
+  cases n <;> grind [Rci.iter]
+
+@[grind =]
+theorem Nat.toList_take_zero_iter_rci {m : Nat} :
+    ((m...*).iter.take 0).toList = [] := by
+  rw [Nat.toList_take_iter_rci_eq_match]
+
+@[grind =]
+theorem Nat.toList_take_add_one_iter_rci {m n : Nat} :
+    ((m...*).iter.take (n + 1)).toList = m :: (((m + 1)...*).iter.take n).toList := by
+  rw [Nat.toList_take_iter_rci_eq_match]
+
+@[grind =]
+theorem Nat.toList_rco_self {m : Nat} :
+    (m...m).toList = [] := by
+  simp [toList_rco_eq_nil]
+
+@[grind =]
+theorem Nat.toList_take_iter_rci {m n : Nat} :
+    (((m : Nat)...*).iter.take n).toList = ((m : Nat)...(m + n : Nat)).toList := by
+  induction n generalizing m <;> grind [Nat.toList_rco_eq_cons, Nat.toList_take_add_one_iter_rci]
+
+@[grind =]
+theorem List.map_swap_zip {xs : List α} {ys : List β} :
+    (ys.zip xs).map Prod.swap = xs.zip ys := by
+  induction xs generalizing ys
+  · grind [zip_nil_right, zip_nil_left]
+  · cases ys
+    · grind [zip_nil_left, zip_nil_right]
+    · grind [zip_cons_cons, Prod.swap_prod_mk]
+
+theorem solution_spec {xs : List Int} :
+    solution xs = (xs.mapIdx (fun i x => if i % 2 = 0 then x else 0)).sum :=
+  match xs with
+  | [] => by
+    simp [solution, ← Iter.foldl_toList]
+    rw [Iter.toList_zip_of_finite_right]
+    grind [List.toList_iter, List.length_nil, List.zip_nil_right]
+  | [x] => by
+    simp [solution, ← Iter.foldl_toList]
+    rw [Iter.toList_zip_of_finite_right]
+    simp [Nat.toList_take_iter_rci]
+  | x :: y :: xs => by
+    have := solution_spec (xs := xs)
+    simp [solution, ← Iter.foldl_toList] at this ⊢
+    rw [Iter.toList_zip_of_finite_right]
+    simp [Nat.toList_take_iter_rci, Nat.toList_rco_eq_cons]
+    -- ugh, foldr would have been nicer
+
+
+theorem solution_spec {xs : List Int} :
+    solution xs = (xs.mapIdx (fun i x => if i % 2 = 0 then x else 0)).sum := by
+  simp [solution, ← Iter.foldl_toList]
+  rw [Iter.toList_zip_of_finite_right]
+  simp [Nat.toList_take_iter_rci]
+  rw [List.mapIdx_eq_zipIdx_map, List.zipIdx_eq_zip_range', List.range'_eq_toList_rco]
+  simp
+  rw [← List.map_swap_zip]
+  induction xs
+  · simp
+  · simp [Nat.toList_rco_eq_cons]
+
 
 /-!
 ## Prompt
@@ -8,7 +118,7 @@ def solution : Unit :=
 
 def solution(lst):
     """Given a non-empty list of integers, return the sum of all of the odd elements that are in even positions.
-    
+
 
     Examples
     solution([5, 8, 7, 1]) ==> 12
